cleaner API

theories/util.v
@@ -7,31 +7,36 @@ Section lift.
   Notation paddr := N.
   Variable byte_at : forall (hpa:paddr) (hpaFrac : Qp) (value : N), PROP.
 
-  Fixpoint lift n (pa : paddr) (q:Qp) (v : N) :=
+  Fixpoint lift_aux n (pa : paddr) (q:Qp) (v : N) :=
     match n with
     | O => byte_at pa q v
     | S n => let bytesize :N := (2^(N.of_nat n)) in
             let bitsize := (8*bytesize)%N in
-            lift n pa q (N.land v (2^bitsize - 1))
-            ** lift n (pa+bytesize) q (N.shiftr v bitsize)
+            lift_aux n pa q (N.land v (2^bitsize - 1))
+            ** lift_aux n (pa+bytesize) q (N.shiftr v bitsize)
     end.
+
+  Definition lift (nbytes:N) (pa : paddr) (q:Qp) (v : N) :=
+    lift_aux (N.to_nat (BinNatDef.N.log2 nbytes)) pa q v.
 
   Section test.
 
-    Local Definition short_at (pa : paddr) (q:Qp) (v : N) : PROP :=
-      byte_at pa q (N.land v (2^8 - 1))%N **
-              byte_at (pa + 1)%N q (N.shiftr v 8).
+    Let short_at (pa : paddr) (q:Qp) (v : N) : PROP :=
+      byte_at pa q (N.land v (2^8 - 1))%N
+      ** byte_at (pa + 1)%N q (N.shiftr v 8).
 
-    Local Definition word_at (pa : paddr) (q : Qp) (v : N) : PROP :=
-      short_at pa q (N.land v (2^16 - 1))**
-               short_at (pa + 2)%N q (N.shiftr v 16).
+    Let word_at (pa : paddr) (q : Qp) (v : N) : PROP :=
+      short_at pa q (N.land v (2^16 - 1))
+      ** short_at (pa + 2)%N q (N.shiftr v 16).
 
-    Example t1 pa q v : short_at pa q v = lift 1 pa q v.
-    reflexivity.
-    Qed.
-    Example t2 pa q v : word_at pa q v = lift 2 pa q v.
-    reflexivity.
-    Qed.
+    Example t1 pa q v : short_at pa q v = lift 2 pa q v.
+    Proof.
+      reflexivity.
+    Abort.
+    Example t2 pa q v : word_at pa q v = lift 4 pa q v.
+    Proof.
+      reflexivity.
+    Abort.
   End test.
 
 End lift.
